theories/Operational/Common/OSAdmissibleCandidateSourceContract.v
@@ -1,0 +1,156 @@
+From Stdlib Require Import List.
+Import ListNotations.
+From RocqSched Require Import Foundation.Base.
+From RocqSched Require Import Semantics.Schedule.
+From RocqSched Require Import Abstractions.SchedulingAlgorithm.SchedulerBridge.
+From RocqSched Require Import Multicore.Common.MultiCoreBase.
+From RocqSched Require Import Multicore.Common.Admissibility.
+From RocqSched Require Import Operational.Common.OSProjectionInterface.
+From RocqSched Require Import Operational.Common.ConcreteExecution.
+From RocqSched Require Import Operational.Common.Projection.
+From RocqSched Require Import Operational.Common.OSCandidateSourceContract.
+From RocqSched Require Import Operational.Common.OSLocalAdapterContract.
+
+Record labeled_concrete_admissible_candidate_source_contract
+    {CState : Type}
+    {P : OSLabeledProjection CState}
+    (J : JobId -> Prop)
+    (jobs : JobId -> Job)
+    (adm : admissible_cpu)
+    (m : nat)
+    (candidates_of : CandidateSource)
+    (ex : labeled_concrete_execution P m) : Prop :=
+  mkLabeledConcreteAdmissibleCandidateSourceContract {
+    lcacsc_base :
+      labeled_concrete_candidate_source_contract
+        jobs
+        m
+        candidates_of
+        ex;
+    lcacsc_candidates_sound :
+      forall t j,
+        In j (projected_candidate_list jobs m ex candidates_of t) ->
+        J j;
+    lcacsc_candidates_complete :
+      forall t j,
+        J j ->
+        eligible
+          jobs
+          m
+          (project_schedule (osl_to_op_trace P (lce_trace ex)))
+          j
+          t ->
+        admissible_somewhere
+          adm
+          jobs
+          m
+          (project_schedule (osl_to_op_trace P (lce_trace ex)))
+          j
+          t ->
+        In j (projected_candidate_list jobs m ex candidates_of t);
+  }.
+
+Arguments lcacsc_base
+  {CState P J jobs adm m candidates_of ex} _.
+Arguments lcacsc_candidates_sound
+  {CState P J jobs adm m candidates_of ex} _ _ _ _.
+Arguments lcacsc_candidates_complete
+  {CState P J jobs adm m candidates_of ex} _ _ _ _ _ _.
+
+Record labeled_concrete_strong_admissible_candidate_source_contract
+    {CState : Type}
+    {P : OSLabeledProjection CState}
+    (J : JobId -> Prop)
+    (jobs : JobId -> Job)
+    (adm : admissible_cpu)
+    (m : nat)
+    (candidates_of : CandidateSource)
+    (ex : labeled_concrete_execution P m) : Prop :=
+  mkLabeledConcreteStrongAdmissibleCandidateSourceContract {
+    lcsacsc_base :
+      labeled_concrete_admissible_candidate_source_contract
+        J
+        jobs
+        adm
+        m
+        candidates_of
+        ex;
+    lcsacsc_candidates_somewhere :
+      forall t j,
+        In j (projected_candidate_list jobs m ex candidates_of t) ->
+        admissible_somewhere
+          adm
+          jobs
+          m
+          (project_schedule (osl_to_op_trace P (lce_trace ex)))
+          j
+          t;
+  }.
+
+Arguments lcsacsc_base
+  {CState P J jobs adm m candidates_of ex} _.
+Arguments lcsacsc_candidates_somewhere
+  {CState P J jobs adm m candidates_of ex} _ _ _ _.
+
+Record os_local_admissible_candidate_source_adapter_contract
+    {CState : Type}
+    (P : OSLabeledProjection CState)
+    (J : JobId -> Prop)
+    (candidates_of : CandidateSource)
+    (jobs : JobId -> Job)
+    (adm : admissible_cpu)
+    (m : nat) : Type :=
+  mkOSLocalAdmissibleCandidateSourceAdapterContract {
+    olacsc_base :
+      os_local_candidate_source_adapter_contract
+        P
+        candidates_of
+        jobs
+        adm
+        m;
+    olacsc_admissible :
+      labeled_concrete_admissible_candidate_source_contract
+        J
+        jobs
+        adm
+        m
+        candidates_of
+        (olac_execution (olcsac_base olacsc_base));
+  }.
+
+Arguments olacsc_base
+  {CState P J candidates_of jobs adm m} _.
+Arguments olacsc_admissible
+  {CState P J candidates_of jobs adm m} _.
+
+Record os_local_strong_admissible_candidate_source_adapter_contract
+    {CState : Type}
+    (P : OSLabeledProjection CState)
+    (J : JobId -> Prop)
+    (candidates_of : CandidateSource)
+    (jobs : JobId -> Job)
+    (adm : admissible_cpu)
+    (m : nat) : Type :=
+  mkOSLocalStrongAdmissibleCandidateSourceAdapterContract {
+    olsacsc_base :
+      os_local_admissible_candidate_source_adapter_contract
+        P
+        J
+        candidates_of
+        jobs
+        adm
+        m;
+    olsacsc_strong :
+      labeled_concrete_strong_admissible_candidate_source_contract
+        J
+        jobs
+        adm
+        m
+        candidates_of
+        (olac_execution (olcsac_base (olacsc_base olsacsc_base)));
+  }.
+
+Arguments olsacsc_base
+  {CState P J candidates_of jobs adm m} _.
+Arguments olsacsc_strong
+  {CState P J candidates_of jobs adm m} _.
